<!--
 * @Author: Uper 41718895+Hyliu-BUAA@users.noreply.github.com
 * @Date: 2022-06-28 18:24:56
 * @LastEditors: Uper 41718895+Hyliu-BUAA@users.noreply.github.com
 * @LastEditTime: 2022-07-17 22:52:32
 * @FilePath: /Quantum_Mechanics/qm/5.幺正算符.md
 * @Description: 这是默认设置,请设置`customMade`, 打开koroFileHeader查看配置 进行设置: https://github.com/OBKoro1/koro1FileHeader/wiki/%E9%85%8D%E7%BD%
-->
# 1. 幺正算符 (`Unitary operator`)
<font color="73DB90" size="4">

满足下列三个条件之一的算符 $\^{U}$ 称为幺正算符：
1. $\^{U}^{\dagger} = \^{U}^{-1}$，即 $\^{U}^{\dagger}\^{U} = \^{U}\^{U}^{\dagger} = \^{I}$
2. 对一切左矢$\bra{\phi}$和右矢$\ket{\psi}$，$\^{U}$满足：
$$ \braket{\^{U}\phi|\^{U}\psi} = \braket{\phi|\psi} $$
3. $\ket{U\psi} = \ket{\psi}$，对一切$\ket{\psi}$成立

</font>


# 2. 幺正变换 (`Unitary transform`)
## 2.1. `unitary transformation(酉变化)` 在 QM 中的应用
1. In quantum mechanics, the `Schrodiger equation` describes how a system changes with time. Therefore, once the `Hamiltonian` is known, the time dynamics are in principle known. All that remains is to `plug the Hamiltonian into the Schrödinger equation` and `solve for the system state` as a function of time.
2. <font color="orange" size="4">Often, the `Schrodinger equation` is diffrent to solve. Therefore, physicists apply `unitary transformation` to the Hamiltonian. </font>Doing so can result in a simplified version of the Schrödinger equation which nonetheless `has the same solution as the original`.

<font color="red" size="4">

Note
----
1. 一个孤立体系，不与外界耦合，不被测量，被演化的过程称为`幺正变换`。
2. `幺正变换`过程中没有信息的流出，该烟花过程可逆。
3. 按照薛定谔方程演化叫做`幺正变换`，一般叫做`U过程`。`波函数坍缩`是非幺正的，一般叫做`R过程`

</font>

## 2.2. Product of two `unitary operators`
### 2.2.1. 内容
$$\begin{cases}
(\^{U}\^{V})^{\dagger}(\^{U}\^{V}) = I \\
(\^{U}\^{V})(\^{U}\^{V})^{\dagger} = I
\end{cases}$$

### 2.2.2. Proof
1. If $\^{U}, \^{V}$ are `unitary operator`. <font color="73DB90" size="4">(`Hamiltonian` of Operator is equal to `inverse element` of operator.)</font>
$$\begin{cases}
\^{U}^{-1} = \^{U}^{\dagger}    \\
\^{V}^{-1} = \^{V}^{\dagger}
\end{cases}$$
2. Product of two unitary operators:
$$\begin{cases}
(\^{U}\^{V})^{\dagger}(\^{U}\^{V}) = \^{V}^{\dagger}\^{U}^{\dagger}\^{U}\^{V} = I \\
(\^{U}\^{V})(\^{U}\^{V})^{\dagger} = \^{U}\^{V}\^{V}^{\dagger}\^{U}^{\dagger=} = I
\end{cases}$$


## 2.3. `Eigenvalue magnitude` of unitary operators
### 2.3.1. 内容
<font color="73DB90" size="4">

1. The `eigenval` of a `unitary operator` are numbers of `magnitude 1`

</font>

### 2.3.2. Proof
1. $\^{U}$ is `unitary operator`, so
$$\begin{aligned}
\^{U}\ket{\psi} = u\ket{\psi}
\end{aligned}$$
2. According to the attribution of `unitary operator`:
$$\begin{aligned}
\braket{\psi|\psi} = \braket{\^{U}\psi|\^{U}\psi} = u^* u\braket{\psi|\psi}
\end{aligned}$$
3. Because $\braket{\psi|\psi} \neq 0$, so
$$\begin{aligned}
u^* u = 1 \rightarrow |u| = 1
\end{aligned}$$


## 2.4. `Eigenstate` of unitary operator
### 2.4.1. 内容
<font color="73DB90" size="4">

1. At the `eigenstate` of `unitary operator` that corresponds to different eigenvalues are `orthogonal`.

</font>

### 2.4.2. Prerequisites
1. Real space:
$$\^{U}^{\dagger}\ket{\lambda} = \lambda^*\ket{\lambda}$$
2. Dual space:
$$\bra{\lambda}\^{U} = \lambda\bra{\lambda}$$

### 2.4.3. Proof
1. Formula 1:
$$\begin{cases}
\braket{\mu|\^{U}|\lambda} = \lambda\braket{\mu|\lambda}    \\
\braket{\mu|\^{U}|\lambda} = \mu\braket{\mu|\lambda}
\end{cases}$$
2. Substract 1 and 2:
$$\begin{aligned}
(\lambda-\mu)\braket{\mu|\lambda} = 0
\end{aligned}$$
3. $\lambda \neq \mu$, so, 
$$\begin{aligned}
<\mu | \lambda> = 0
\end{aligned}$$

## 2.5. `Unitary transformation` `conserve` the `scalar product`
### 2.5.1. 内容
<font color="73DB90" size="4">

$$\braket{ \psi_1^{'} | \psi_2^{'} } = \braket{ \psi_1 | \psi_2 } $$

</font>

### 2.5.2. Proof
$$\begin{aligned}
\braket{ \psi_1^{'} | \psi_2^{'} } = \braket{ \psi_1 | \^{U}^{\dagger}\^{U} | \psi_2 } = \braket{\psi_1 | \psi_2}
\end{aligned}$$

## 2.6. `Unitary transformations` on operators
### 2.6.1. 内容
<font color="73DB90" size="4">

1. 算符的幺正变换：
- $ \^{A} \rightarrow \^{A^{'}} $
- $ \^{A} = \^{U^{\dagger}}\^{A^{'}}\^{U} $
- $ \^{A^{\dagger}} = \^{U}\^{A}\^{U^{\dagger}} $

</font>

### 2.6.2. Prequisite
1. $\{ \ket{v_m} \} \rightarrow \{ \ket{v_m^{'}}=\^{U}\ket{v_m} \}$

### 2.6.3. Proof
1. Step 1:
$$\begin{cases}
\braket{v_m^{'}|\^{A^{'}}|v_m^{'}} = \braket{v_m|\^{A}|v_m} \\
\braket{v_m^{'}|\^{A^{'}}|v_m^{'}} = \braket{v_m|\^{U}^{\dagger}\^{A^{'}}\^{U}|v_m}
\end{cases}$$
2. So:
$$\begin{aligned}
\^{A} = \^{U^{\dagger}}\^{A^{'}}\^{U}
\end{aligned}$$
3. Multiply $\^{U}$ and $\^{U^{\dagger}}$:
$$\begin{aligned}
\^{A^{'}} = \^{U}\^{A}\^{U^{\dagger}}
\end{aligned}$$